devel/Iron/SystemF2Effect/Step/Progress.v
@@ -1,5 +1,7 @@
 
 Require Export Iron.SystemF2Effect.Step.TypeC.
+Require Export Iron.SystemF2Effect.Store.LiveE.
+Require Export Iron.SystemF2Effect.Store.LiveS.
 
 
 Definition done (fs : stack) (x : exp)
@@ -10,48 +12,59 @@ Definition done (fs : stack) (x : exp)
    Also add this condition to preservation to get region deallocation. *)
 Lemma progress
  :  forall se ss sp fs x1 t1 e1
- ,  WfFS   se sp ss fs
- -> TYPEC  nil nil se sp fs x1 t1 e1
+ ,   WfFS   se sp ss fs
+ ->  LiveS  ss fs -> LiveE fs e1
+ ->  TYPEC  nil nil se sp fs x1 t1 e1
  ->  done fs x1
   \/ (exists ss' sp' fs' x1', STEPF ss sp fs x1 ss' sp' fs' x1').
 Proof.
- intros se ss sp fs x1 t1 e1 HW HC.
+ intros se ss sp fs x1 t1 e1 HW HLS HLE HC.
  gen t1 e1.
  induction x1; intros; eauto.
- 
+
+
+ (*********************************************************)
  Case "XVal".
-  induction fs.
-  SCase "fs = nil".
-   left.
-   unfold done. rip. exists v. auto.
+ { induction fs.
+   SCase "fs = nil".
+    left.
+    unfold done. rip. exists v. auto.
 
-  SCase "fs = cons ...".
-   right.
-   destruct a as [t x | n].
-   SSCase "FLet".
-    exists ss. exists sp. exists fs. exists (substVX 0 v x).
-    eauto.
-   SSCase "FUse".
-    exists ss. exists sp. exists fs. exists (XVal v).
-    eauto.
+   SCase "fs = cons ...".
+    right.
+    destruct a as [t x | n].
+    SSCase "FLet".
+     exists ss. exists sp. exists fs. exists (substVX 0 v x).
+     eauto.
+    SSCase "FUse".
+     exists ss. exists sp. exists fs. exists (XVal v).
+     eauto.
+ }
 
+
+ (*********************************************************)
  Case "XLet".
-  right.
-  exists ss. exists sp. exists (fs :> FLet t x1_2). exists x1_1.
-  eauto.
+ { right.
+   exists ss. exists sp. exists (fs :> FLet t x1_2). exists x1_1.
+   eauto.
+ }
 
+
+ (*********************************************************)
  Case "XApp".
-  right.
-  exists ss. exists sp. exists fs.
-  inverts_typec.
-  destruct v; nope.
-  SCase "v1 = XLam".
-   exists (substVX 0 v0 e). eauto.
-  SCase "v1 = XConst".
-   destruct c; nope.
+ { right.
+   exists ss. exists sp. exists fs.
+   inverts_typec.
+   destruct v; nope.
+   SCase "v1 = XLam".
+    exists (substVX 0 v0 e). eauto.
+   SCase "v1 = XConst".
+    destruct c; nope.
+ }
 
+ (*********************************************************)
  Case "XAPP".
-  right.  
+ { right.  
    exists ss. exists sp. exists fs.
    inverts_typec.
    destruct v; nope.
@@ -59,75 +72,116 @@ Proof.
     exists (substTX 0 t e). eauto.
    SCase "v1 = XConst".
     destruct c; nope.
+ }
 
+
+ (*********************************************************)
  Case "XOp1".
-  right.
-  exists ss. exists sp. exists fs.
-  destruct o.
-  SCase "OSucc".
-   inverts_typec.
-   snorm. inverts H8.
-   destruct v; nope.
-   destruct c; nope.
-   eauto.
- SCase "OIsZero".
-   inverts_typec.
-   snorm. inverts H8.
-   destruct v; nope.
-   destruct c; nope.
-   eauto.
+ { right.
+   exists ss. exists sp. exists fs.
+   destruct o.
+   SCase "OSucc".
+    inverts_typec.
+    snorm. inverts H8.
+    destruct v; nope.
+    destruct c; nope.
+    eauto.
+  SCase "OIsZero".
+    inverts_typec.
+    snorm. inverts H8.
+    destruct v; nope.
+    destruct c; nope.
+    eauto.
+ }
 
+
+ (*********************************************************)
  Case "XNew".
-  right.
-  exists ss. 
-  exists (sp :> SRegion (allocRegion sp)). 
-  exists (fs :> FUse    (allocRegion sp)).
-  eauto.
+ { right.
+   exists ss. 
+   exists (sp :> SRegion (allocRegion sp)). 
+   exists (fs :> FUse    (allocRegion sp)).
+   eauto.
+ }
 
+
+ (*********************************************************)
  Case "XAlloc".
-  right. 
-  inverts_typec. 
-  have HR: (exists n, t = TCap (TyCapRegion n)).
-  destruct HR as [n].
-  exists (StValue n v <: ss).
-  exists sp.
-  exists fs.
-  exists (XVal (VLoc (length ss))).
-  subst. auto.
+ { right. 
+   inverts_typec. 
+   have HR: (exists n, t = TCap (TyCapRegion n)).
+   destruct HR as [n].
+   exists (StValue n v <: ss).
+   exists sp.
+   exists fs.
+   exists (XVal (VLoc (length ss))).
+   subst. auto.
+ }
 
+
+ (*********************************************************)
  Case "XRead".
-  right.
-  inverts HC. inverts_type.
-  have HR: (exists n, t = TCap (TyCapRegion n)).
-  destruct HR as [n]. subst.
+ { right.
+   inverts HC. inverts_type.
+   have HR: (exists n, t = TCap (TyCapRegion n)).
+   destruct HR as [n]. subst.
 
-  assert (exists l, v = VLoc l) as HL.
+   assert (exists l, v = VLoc l) as HL.
+    destruct v; burn.
+    destruct c; nope.
+   dest l. subst.
+
+   inverts_type. inverts HW. 
+   exists ss. exists sp. exists fs.
+   rip.
+
+   (* There is a binding in the store corresponding
+      to the entry in the store environment. *)
+   have (exists b, get l ss = Some b).
+    dest b.
+
+   unfold STORET in *.
+
+   destruct b.
+   (* Store binding contains a value. *)
+   - have HB: (TYPEB nil nil se sp 
+                    (StValue n0 v) 
+                    (TRef (TCap (TyCapRegion n)) t0))
+      by (eapply Forall2_get_get_same; eauto).
+     inverts HB.
+     exists (XVal v).
+     eauto.
+    
+   (* Store binding is dead, 
+      can't happen due to binding liveness constraints LiveE/LiveE *)
+   - have HB: (TYPEB nil nil se sp
+                     (StDead n0)
+                     (TRef (TCap (TyCapRegion n)) t0))
+      by (eapply Forall2_get_get_same; eauto).
+     inverts HB.
+
+     remember (TCap (TyCapRegion n)) as p. 
+
+     have (SubsT nil sp e1 (TRead p) KEffect)
+      by  (eapply EqSym in H; eauto).
+
+     have (LiveE fs (TRead p)).
+
+     lets D: liveS_liveE_value ss fs (TRead p) l (StDead n).
+     spec D n. rip. subst p. snorm. rip.
+     have (Some n = Some n). rip.
+     have (n = n). rip. nope.
+ }
+
+
+ (*********************************************************)
+ Case "XWrite".
+ { right.
+   inverts_typec.
+   have HR: (exists n, t = TCap (TyCapRegion n)).
+    destruct HR as [n]. subst.
    destruct v; burn.
    destruct c; nope.
-  dest l. subst.
-
-  inverts_type. 
-  exists ss.
-  exists sp.
-  exists fs.
-  inverts HW. rip.
-  have (exists v, get l ss = Some v).
-   dest v.
-
-  unfold STORET in *.
-  destruct v.
-  have HB: (TYPEB nil nil se sp (StValue n0 v) (TRef (TCap (TyCapRegion n)) t0))
-   by (eapply Forall2_get_get_same; eauto).
-  inverts HB.
-  exists (XVal v).
-  eauto.
-
- Case "XWrite".
-  right.
-  inverts_typec.
-  have HR: (exists n, t = TCap (TyCapRegion n)).
-   destruct HR as [n]. subst.
-  destruct v; burn.
-  destruct c; nope.
+ }
 Qed.
 
