devel/Iron/SystemF2Effect/Store/LiveS.v
@@ -1,0 +1,64 @@
+
+Require Export Iron.SystemF2Effect.Step.Frame.
+Require Export Iron.SystemF2Effect.Store.Bind.
+Require Export Iron.SystemF2Effect.Store.LiveE.
+
+
+Definition isFUse    (p : nat) (f : frame)
+ := f = FUse p.
+Hint Unfold isFUse.
+
+
+Definition isStValue (b : stbind)
+ := exists p v, b = StValue p v.
+Hint Unfold isStValue.
+
+
+Definition regionOfStBind (b : stbind)
+ := match b with 
+    | StValue n _ => n
+    | StDead  n   => n
+    end.
+Hint Unfold regionOfStBind.
+
+
+Definition LiveF (ss : store) (f : frame)
+ := forall p, isFUse p f 
+           -> Forall (fun b => regionOfStBind b = p
+                            -> isStValue b) 
+                      ss.
+
+Definition LiveS  (ss : store) (fs : stack)
+ := Forall (LiveF ss) fs.
+                         
+
+
+Lemma liveS_liveE_value
+ :  forall ss fs e l b p
+ ,  LiveS ss fs
+ -> LiveE fs e
+ -> handleOfEffect e = Some p
+ -> get l ss         = Some b
+ -> regionOfStBind b = p
+ -> exists v, b = StValue p v.
+Proof.
+ intros ss fs e l b p HLS HLE. intros.
+
+ destruct b.
+ - snorm. subst. exists v. eauto.
+ - have HIF: (In (FUse p) fs) 
+    by  (eapply liveE_fUse_in; eauto; snorm).
+
+   unfold LiveS in HLS.
+   unfold LiveF in HLS.
+   snorm.
+ 
+   eapply HLS with (p := n) in HIF.
+   + snorm.
+     have (In (StDead n) ss) as HD. subst.
+     eapply HIF in HD.
+     unfold isStValue in HD. nope.
+     snorm.
+   + snorm.
+Qed.
+
